iris/proofmode/class_instances_cmra.v
@@ -2,25 +2,25 @@ From iris.proofmode Require Import modality_instances classes.
 Import bi.
 
 Section class_instances_cmra_valid.
-  Context `{!Sbi PROP}.
+  Context {SI : sidx} `{!Sbi PROP}.
 
   Global Instance into_pure_internal_cmra_valid `{!CmraDiscrete A} (a : A) :
-    @IntoPure PROP (✓ a) (✓ a).
+    @IntoPure _ PROP (✓ a) (✓ a).
   Proof. by rewrite /IntoPure internal_cmra_valid_discrete. Qed.
 
   Global Instance from_pure_internal_cmra_valid {A : cmra} (a : A) :
-    @FromPure PROP false (✓ a) (✓ a).
+    @FromPure _ PROP false (✓ a) (✓ a).
   Proof.
     rewrite /FromPure /=. apply bi.pure_elim'=> ?.
     rewrite -internal_cmra_valid_intro //.
   Qed.
 
   Global Instance into_pure_internal_included {A : cmra} (a b : A) `{!Discrete b} :
-    @IntoPure PROP (a ≼ b) (a ≼ b).
+    @IntoPure _ PROP (a ≼ b) (a ≼ b).
   Proof. by rewrite /IntoPure internal_included_discrete. Qed.
 
   Global Instance from_pure_internal_included {A : cmra} (a b : A) :
-    @FromPure PROP false (a ≼ b) (a ≼ b).
+    @FromPure _ PROP false (a ≼ b) (a ≼ b).
   Proof.
     rewrite /FromPure /=. apply bi.pure_elim'=> ?.
     rewrite -internal_included_intro //.
