iris/proofmode/class_instances_embedding.v
@@ -6,13 +6,13 @@ Import bi.
 instance is not used when there is no embedding between [PROP] and [PROP']. The
 first [`{BiEmbed PROP PROP'}] is not considered as a premise by Rocq TC search
 mechanism because the rest of the hypothesis is dependent on it. *)
-Global Instance as_emp_valid_embed `{!BiEmbed PROP PROP'} d (φ : Prop) (P : PROP) :
+Global Instance as_emp_valid_embed {SI : sidx} `{!BiEmbed PROP PROP'} d (φ : Prop) (P : PROP) :
   BiEmbed PROP PROP' →
   AsEmpValid0 d φ P → AsEmpValid d φ ⎡P⎤.
 Proof. rewrite /AsEmpValid0 /AsEmpValid=> _ [? ?]. rewrite embed_emp_valid //. Qed.
 
 Section class_instances_embedding.
-Context `{!BiEmbed PROP PROP'}.
+Context {SI : sidx} {PROP PROP' : bi} `{!BiEmbed PROP PROP'}.
 Implicit Types P Q R : PROP.
 
 Global Instance into_pure_embed P φ :
@@ -32,7 +32,7 @@ Qed.
 (* When having a modality nested in an embedding, e.g. [ ⎡|==> P⎤ ], we prefer
 the embedding over the modality. *)
 Global Instance from_modal_embed P :
-  FromModal True (@modality_embed PROP PROP' _) ⎡P⎤ ⎡P⎤ P.
+  FromModal True (@modality_embed SI PROP PROP' _) ⎡P⎤ ⎡P⎤ P.
 Proof. by rewrite /FromModal. Qed.
 
 Global Instance from_modal_id_embed φ `(sel : A) P Q :
